Chore: Refactor Aka

Straume/Aka.lean
@@ -2,25 +2,41 @@ import Straume.Chunk
 import Straume.Coco
 import Straume.Flood
 import Straume.Iterator
-import Straume.Zeptoparsec
+
+/-!
+## The Aka class
+This module is designed first and foremost to provide Megaparsec users
+with a way to work with greater-than-RAM and infinite streams.
+-/
 
 open Straume.Chunk (Chunk Terminable coreturn)
 open Straume.Coco (Coco)
 open Straume.Flood (Flood)
-open Straume.Iterator (Iterable iter)
-open Straume.Iterator (Bijection)
-open Zeptoparsec renaming Parsec → Zepto.Parsec
-open Zeptoparsec renaming ParseResult → Zepto.Res
+open Straume.Iterator (Iterable iter Bijection)
 
+universe u v
 
-/-
-  This module is designed first and foremost to provide Megaparsec users
-  with a way to work with greater-than-RAM and infinite streams.
+-------------------------------
+----       Aka class       ----
+-------------------------------
+
+/--
+A way to read atomic values `v` out of a source `s`,
+which emits `Iterable α v`.
+The information about finality is tacked onto the values of type `v`
+via type `f`.
+An example of such `f` is `Chunk`.
 -/
-namespace Straume.Aka
+class Straume.Aka (m : Type u → Type v)
+          (s : Type u)
+          (f : Type u → Type u)
+          (v : Type u) where
+                        -- TODO: Can we express _buffer > 0 in types?
+  take1 (_source : s) (_buffer : Nat := 2048) : m ((f v) × s)
 
-universe u
-universe v
+section aka_instance
+
+namespace Straume.Aka
 
 -- class Stream (S : Type) where
 --   Token : Type
@@ -34,15 +50,16 @@ universe v
 --   take1 : S → Option (Token × S)
 --   takeN : Nat → S → Option (Chunk \a × S)
 --   takeWhile : (Token → Bool) → S → (Chunk \a × S)
+-- TODO: ^^^^^^^^^ Keep this?
 
 -------------------------------
 ----         takeN         ----
 -------------------------------
 
-def takeN {f : Type u → Type u} {α β : Type u}
-          (n : Nat) (src : s) (b : Nat := 2048)
-          [Coco α s] [Flood m s] [Terminable f] [Monad m] [Iterable α β]
-          : m (f α × s) := do
+variable {f : Type u → Type u} {α β s : Type u} {m : Type u → Type v} (src : s) 
+         [Coco α s] [Flood m s] [Terminable f] [Monad m] [Iterable α β]
+
+def takeN (n : Nat) (b : Nat := 2048) : m (f α × s) := do
   -- BEST EFFORT
   let l := Iterable.length (Coco.coco src : α)
   let srcₑ ← Flood.flood src $ max b ((n - l) + 1) -- We expand the buffer
@@ -64,27 +81,37 @@ def takeN {f : Type u → Type u} {α β : Type u}
 ----         take1         ----
 -------------------------------
 
--- We use `takeN` to snip off `α` of length 1 and then use
--- `Iterable` to take the first (and only) element.
-def take1 {f : Type u → Type u} {α β : Type u}
-          (src : s) (b := 2048)
-          [Coco α s] [Flood m s] [Terminable f] [Monad m]
-          [Iterable α β] [Bijection β α] : m ((f β) × s) :=
-  takeN 1 src b >>= fun ((y : f α), s₁) =>
+instance : Aka m s f β where
+  -- We use `takeN` to snip off `α` of length 1 and then use
+  -- `Iterable` to take the first (and only) element.
+  take1 src b := takeN src 1 b >>= 
+    fun ((y : f α), s₁) =>
     pure ((Iterable.curr ∘ iter) <$> y, s₁)
 
+example : Aka IO (String × IO.FS.Handle) Chunk Char := by infer_instance
+/-^^^^^^^^^^^^^^^^^
+works, for example
+TODO: Delete this comment
+-/
+
+end Straume.Aka
+
+end aka_instance
 
 -------------------------------
 ----       takeWhile       ----
 -------------------------------
 
-private partial def takeWhileDo
-    {f : Type u → Type u} {α β : Type u}
-    (φ : β → Bool) (stream₀ : s) (b : Nat) (acc : f α)
-    [Coco α s] [Iterable α β] [Terminable f] [Monad m]
-    [Inhabited (m (f α × s))] [Inhabited α] [Flood m s]
+section aka_takeWhile
+
+namespace Straume.Aka
+  
+variable {f : Type u → Type u} {α β s : Type u} (φ : β → Bool) 
+         [Coco α s] [Iterable α β] [Terminable f] [Monad m] [Inhabited α] [Flood m s]
+
+private partial def takeWhileDo (stream₀ : s) (b : Nat) (acc : f α) [Inhabited (m (f α × s))] 
     : m (f α × s) := do
-  let ((atom : f β), stream) ← take1 stream₀ b
+  let ((atom : f β), stream) ← Aka.take1 stream₀ b
   match Terminable.un atom with
   | .none => pure (acc, stream₀)
   | .some c =>
@@ -92,7 +119,7 @@ private partial def takeWhileDo
       match (Terminable.reason acc, Terminable.reason atom) with
       -- cont cases
       | (.none, .none) =>
-        takeWhileDo φ stream b $
+        takeWhileDo stream b $
           Terminable.mkCont $ Iterable.push (coreturn acc) c
       -- fin cases
       | (.none, .some ()) =>
@@ -102,46 +129,30 @@ private partial def takeWhileDo
     else
       pure (acc, stream₀)
 
-partial def takeWhile
-    {f : Type u → Type u} {α β : Type u}
-    (φ : β → Bool) (src : s) (b : Nat := 2048)
-    [Coco α s] [Iterable α β] [Terminable f] [Monad m]
-    [Inhabited (m (f α × s))] [Inhabited α] [Flood m s]
-    : m (f α × s) :=
+partial def takeWhile (src : s) (b : Nat := 2048) [Inhabited (m (f α × s))] : m (f α × s) :=
   takeWhileDo φ src b Terminable.mkNil
+ 
+end Straume.Aka
 
-open Straume.Combinators
-#check λs => Straume.Aka.takeWhile (Function.const Bool true) s 2048
-
+end aka_takeWhile
 -------------------------------
 ----      chunkLength      ----
 -------------------------------
 
-def chunkLength (fx : f α) [Terminable f] [Iterable α β] : Nat :=
+section aka_length
+
+namespace Straume.Aka
+
+variable (fx : f α) [Terminable f] [Iterable α β]
+
+def chunkLength : Nat :=
   match (Terminable.un fx) with
   | .none => 0
   | .some e => Iterable.length e
 
-def storeLength (fx : f α) [Terminable f] [Iterable α β] : f Nat :=
+def storeLength : f Nat :=
   Iterable.length <$> fx
 
--------------------------------
-----       Aka class       ----
--------------------------------
+end Straume.Aka
 
-/-
-  A way to read atomic values `v` out of a source `s`,
-  which emits `Iterable α v`.
-  The information about finality is tacked onto the values of type `v`
-  via type `f`.
-  An example of such `f` is `Chunk`.
--/
-class Aka (m : Type u → Type v)
-          (s : Type u)
-          (f : Type u → Type u)
-          (v : Type u) where
-                        -- TODO: Can we express _buffer > 0 in types?
-  take1 (_source : s) (_buffer : Nat := 2048) : m ((f v) × s)
-
-instance : Aka IO (String × IO.FS.Handle) Chunk Char where
-  take1 src b := take1 src b
+end aka_length
